\documentclass{article}
\usepackage{epsfig}
\pagestyle{empty}
\begin{document}
$ U(r) = \sum_k A_k r^(n_k-2) exp(-alpha_k r^2) \sum_m |Y_lm \rangle \langle Y_lm| $
\pagebreak

$\sum_m |Y_lm \rangle \langle Y_lm|$
\pagebreak

\[ \chi_{k{*} i}(1) = \int dr_2 \frac{k(2) i(2)}{|r_1-r_2|} \]
\pagebreak

\[ \chi_{ki{*}}(1) = \int dr_2 \frac{k(2) i(2)}{|r_1-r_2|} \]
\pagebreak

\[ \xi_{k{*}i,j}(1) = \chi_{ki}(1) j(1) \]
\pagebreak

\[ \xi_{ki{*},j{*}}(1) = \chi_{k{*}i}(1) j(1) \]
\pagebreak

$(ij|kl)$
\pagebreak

$i>=j$
\pagebreak

$k>=l$
\pagebreak

$(ij|kl)=(kl|ij)$
\pagebreak

\[ f = 2/3 * \omega |<x | \vec \mu | i >| ^2 * 2 \]
\pagebreak

$ x $
\pagebreak

$ i $
\pagebreak

\[ f = 2/(3 * \omega) |<x | \vec p | i >| ^2 * 2 \]
\pagebreak

\[ Int[i,p] = \int \frac{1}{r_{12}} \phi_i(1) * \phi_p(1) \]
\pagebreak

\[ F_{pq} = < x^p_i | F | x^q_i > + < x^p_i | \Gamma^q | \phi_i > \]
\pagebreak

\[ < \vec x^p | \vec x^q > = \sum_i x^p_i x^q_i \]
\pagebreak

\[ f(x,x_{\mathrm{min}},x_{\mathrm{max}}) = \left\{ \begin{array}{ll} x_{\mathrm{min}} & x < x_{\mathrm{min}} p(x,x_{\mathrm{min}},x_{\mathrm{max}}) & x_{\mathrm{min}} \leq x_{\mathrm{max}} x & x_{\mathrm{max}} < x \end{array} \right. \]
\pagebreak

$p(x)$
\pagebreak

$p(x_{min})=x_{min}$
\pagebreak

$p(x_{max})=x_{max}$
\pagebreak

$dp(x_{max})/dx=1$
\pagebreak

$dp(x_{min})/dx=d^2p(x_{min})/dx^2=d^2p(x_{max})/dx^2=0$
\pagebreak

$ E[\rho] = \int \epsilon[\rho(x)] dx$
\pagebreak

$ \rho_{\alpha} $
\pagebreak

$ \sigma_{\alpha\alpha} = \nabla \rho_{\alpha}.\nabla \rho_{\alpha} $
\pagebreak

$ \rho_{\beta} $
\pagebreak

$ \sigma_{\alpha\beta} = \nabla \rho_{\alpha}.\nabla \rho_{\beta} $
\pagebreak

$ \sigma_{\beta\beta} = \nabla \rho_{\beta}.\nabla \rho_{\beta} $
\pagebreak

$ \sigma_{\mu \nu} = \nabla \rho_{\mu} . \nabla \rho_{\nu} $
\pagebreak

$ \mu, \nu = \alpha$
\pagebreak

$ \beta $
\pagebreak

$ < \phi | \hat V | \psi > = \int \left( \frac{\partial \epsilon}{\partial \rho_{\alpha}} \phi \psi + \left( 2 \frac{\partial \epsilon}{\partial \sigma_{\alpha \alpha}} + \frac{\partial \epsilon}{\partial \sigma_{\alpha \beta}} \right) \nabla \rho_{\alpha} . \nabla \left( \phi \psi \right) \right) dx $
\pagebreak

$ < \phi_{\alpha} | \hat V | \psi_{\alpha} > = \int \left( \frac{\partial \epsilon}{\partial \rho_{\alpha}} \phi \psi + \left( 2 \frac{\partial \epsilon}{\partial \sigma_{\alpha \alpha}} \nabla \rho_{\alpha} + \frac{\partial \epsilon}{\partial \sigma_{\alpha \beta}} \nabla \rho_{\beta} \right) . \nabla \left( \phi \psi \right) \right) dx $
\pagebreak

$ V_{\alpha} = \frac{\partial \epsilon}{\partial \rho_{\alpha}} - \left(\nabla . \left(2 \frac{\partial \epsilon}{\partial \sigma_{\alpha \alpha}} \nabla \rho_{\alpha} + \frac{\partial \epsilon}{\partial \sigma_{\alpha \beta}} \nabla \rho_{\beta} \right) \right) $
\pagebreak

$ \frac{\partial \epsilon}{\partial \rho_{\alpha}}$
\pagebreak

$ 2 \frac{\partial \epsilon}{\partial \sigma_{\alpha \alpha}} + \frac{\partial \epsilon}{\partial \sigma_{\alpha \beta}}$
\pagebreak

$ \frac{\partial \epsilon}{\partial \rho_{\beta}}$
\pagebreak

$ \frac{\partial \epsilon}{\partial \sigma_{\alpha \alpha}} $
\pagebreak

$ \frac{\partial \epsilon}{\partial \sigma_{\alpha \beta}} $
\pagebreak

$ \frac{\partial \epsilon}{\partial \sigma_{\beta \beta}} $
\pagebreak

\[ f(x,x_{\mathrm{min}},x_{\mathrm{max}}) = \left\{ \begin{array}{ll} x_{\mathrm{min}} & x < x_{\mathrm{min}} \\ p(x,x_{\mathrm{min}},x_{\mathrm{max}}) & x_{\mathrm{min}} \leq x_{\mathrm{max}} \\ x & x_{\mathrm{max}} < x \end{array} \right. \]
\pagebreak

\[ c^2 = a^2 + b^2 \]
\pagebreak

\[ z = frac{x}{1 - y^2} \]
\pagebreak

\[ \nabla^2 u - p(\varepsilon) S (u-g) = \varphi f, \]
\pagebreak

$u$
\pagebreak

$\varepsilon$
\pagebreak

$p(\varepsilon)$
\pagebreak

$2/\varepsilon$
\pagebreak

$S$
\pagebreak

$g$
\pagebreak

$\varphi$
\pagebreak

$f$
\pagebreak

$R$
\pagebreak

$g = Y_0^0$
\pagebreak

$g = Y_1^0$
\pagebreak

$g = Y_2^0$
\pagebreak

$ f = 1 $
\pagebreak

$-G$
\pagebreak

$ e^2 \frac{hope}{despair} $
\pagebreak

\[ \left( -\frac{1}{2} \nabla^2 + V(r) \right) \psi(r) = E \psi(r) \]
\pagebreak

\[ V(r) = \frac{1}{2} |r|^2 \]
\pagebreak

\[ \psi(r) = \left( -\frac{1}{2} \nabla^2 - E \right)^{-1} V(r) \psi(r) \]
\pagebreak

\[ \left(-\nabla^2 + \mu^2 \right) G(r,r'; \mu) = \delta(r-r') \]
\pagebreak

\[ G(r,r'; \mu) = \frac{e^{-\mu |r-r'|}}{4 \pi |r-r|} \]
\pagebreak

$\mu$
\pagebreak

$\mu = \sqrt{-2 E}$
\pagebreak

$\Delta$
\pagebreak

\[ \psi(r) = \left( -\frac{1}{2} \nabla^2 - E + \Delta \right)^{-1} \left( V(r) -\Delta\right) \psi(r) \]
\pagebreak

$\psi(r)=\pi^{-1/4}\exp(-r^2 / 2)$
\pagebreak

$r=$
\pagebreak

$V$
\pagebreak

$Delta$
\pagebreak

$\Delta=7$
\pagebreak

\[ U(r) = \frac{\Delta^2 (r)}{\rho^{2/3} (r)} \]
\pagebreak

$ \Delta $
\pagebreak

$ \rho $
\pagebreak

$ r $
\pagebreak

$ Delta $
\pagebreak

$ \rho() $
\pagebreak

$ rho^{-2/3} $
\pagebreak

$ rho $
\pagebreak

\[ \Delta(r) = exp(- | r | ) \]
\pagebreak

\[ \rho(r) = exp(- 2 | r | ) = \Delta^2(r) \]
\pagebreak

\[ U(r) = \frac{\Delta^2 (r)}{\rho^{2/3} (r)} = exp( - 2 | r | / 3) \]
\pagebreak

$ U(r) $
\pagebreak

\[ \nabla . \left( \epsilon(r) \nabla u(r) \right) = - 4 \pi \rho(r) \]
\pagebreak

\[ \nabla^2 u(r) = - \frac{1}{\epsilon(r)} \left( 4 \pi \rho(r) + \nabla \epsilon(r) . \nabla u(r) \right) \]
\pagebreak

$\rho / \epsilon$
\pagebreak

$\nabla \epsilon . \nabla u / \epsilon$
\pagebreak

$-1 / 4 \pi |r-s|$
\pagebreak

$G(r,s) = 1/|r-s|$
\pagebreak

$-1/4\pi$
\pagebreak

\[ u = G * \left(\rho_{\mbox{vol}} + \rho_{\mbox{surf}} \right) \]
\pagebreak

\[ \rho_{\mbox{vol}} = \frac{\rho}{\epsilon} \]
\pagebreak

\[ \rho_{\mbox{surf}} = \frac{\nabla \epsilon . \nabla u}{4 \pi \epsilon} \]
\pagebreak

$R=2$
\pagebreak

$\epsilon_1 = 1$
\pagebreak

$\epsilon_2 = 10$
\pagebreak

\[ u(r) = \left \lbrace \begin{array}{cc} \frac{1}{\epsilon_2 |r|} & |r| > R \\ \frac{1}{\epsilon_1 |r|} + \left( \frac{1}{\epsilon_2} - \frac{1}{\epsilon_1} \right) \frac{1}{R} & |r| < R \end{array} \right . \]
\pagebreak

\[ q_{\mbox{surface}} = -\frac{\epsilon_2 - \epsilon_1}{\epsilon_2} = -0.9 \]
\pagebreak

$C(r)$
\pagebreak

\[ C(r) = H(R-|r|) \]
\pagebreak

$H(x)$
\pagebreak

\[ \epsilon(r) = \epsilon_1 C(r) + \epsilon_2 \left( 1 - C(r) \right) \]
\pagebreak

\[ H(x,\sigma) = \frac{1}{2} \left( 1 + \mathop{\mathrm{erf}} \frac{x}{\sigma} \right) \]
\pagebreak

$\sigma$
\pagebreak

$\xi=100$
\pagebreak

\[ \rho(r) = \left(\pi \xi \right)^{-3/2} e^{-\xi |r|^2} \]
\pagebreak

$u(r)$
\pagebreak

$m$
\pagebreak

\[ u^{(m+1)} = \alpha u^{(m)} + (1-\alpha) G * \left(\rho^{(m)}_{\mbox{vol}} + \rho^{(m)}_{\mbox{surf}} \right) \]
\pagebreak

$ \alpha \in [0,1]$
\pagebreak

$\alpha$
\pagebreak

$f(r)$
\pagebreak

$d=3$
\pagebreak

$F(x)$
\pagebreak

\[ g(r) = F(f(r)) \]
\pagebreak

\[ \nabla . \left( \epsilon(r) \nabla v(r) \right) = 0 \]
\pagebreak

\[ \nabla^2 v(r) = - \frac{1}{\epsilon} \nabla \epsilon(r) . \nabla v(r) \]
\pagebreak

$-1 / |r-s|$
\pagebreak

$v(\infty)=0$
\pagebreak

$- \partial v / \partial z(\infty) = E$
\pagebreak

$v = - E z$
\pagebreak

\[ v(r) = - E z + u(r) \]
\pagebreak

\[ \nabla^2 u(r) = \frac{1}{\epsilon} \nabla \epsilon(r) . \left(E - \nabla u(r) \right) \]
\pagebreak

$\sigma<0.2$
\pagebreak

$k=8, \mbox{thresh}=1e-5$
\pagebreak

\[ E = \frac{\langle \psi \mid - \frac{1}{2} \nabla^2 - \frac{1}{r} \mid \psi \rangle}{\langle \psi \mid \psi \rangle} \]
\pagebreak

\[ \psi(r) = e^{-r} \]
\pagebreak

$ \psi(\infty)=0 $
\pagebreak

\[ \langle \psi \mid \nabla^2 \mid \psi \rangle = - \langle \nabla \psi \mid \nabla \psi \rangle \]
\pagebreak

$-\frac{1}{2}$
\pagebreak

\[ \frac{\partial u}{\partial t} = c \nabla^2 u(r,t) \]
\pagebreak

\[ \frac{1}{\sqrt{4 \pi c t}} \exp \frac{-x^2}{4 c t} \]
\pagebreak

\[ \frac{\partial u(x,t)}{\partial t} = c \nabla^2 u(x,t) + V_p(x,t) u(x,t) \]
\pagebreak

$ V_p = 0 $
\pagebreak

\[ G_0(x,t) = \frac{1}{\sqrt{4 \pi c t}} \exp \frac{-x^2}{4 c t} \]
\pagebreak

$ V_p $
\pagebreak

\[ G(x,t) = G_0(x,t/2) * \exp(V_p t) * G_0(x,t/2) + O(t^3) \]
\pagebreak

$ V_p(x,t)=\mbox{constant} $
\pagebreak

\begin{eqnarray*} \hat{F} \phi(r) &=& \epsilon \phi(r) \\ \hat{F} &=& -\frac{1}{2} \nabla^2 - \frac{2}{r} + u(r) \\ u(r) &=& \int \frac{\rho(s)}{| r - s |} d^3s \\ \rho(r) &=& \phi(r)^2 \end{eqnarray*}
\pagebreak

$ u(r) $
\pagebreak

$ \rho(r) $
\pagebreak

\[ \phi = - 2 G_{\mu} * ( V \phi) \]
\pagebreak

$ \mu = \sqrt{-2E} $
\pagebreak

$G_{\mu}$
\pagebreak

\[ \left( - \nabla^2 + \mu^2 \right) G(r,r^{\prime}) = \delta(r,r^{\prime}) \]
\pagebreak

$ \exp(-2r) $
\pagebreak

$T~=~-\frac{1}{2} \nabla^2 $
\pagebreak

$ \phi $
\pagebreak

$ <T \phi, \phi > $
\pagebreak

$ < \nabla \phi, \nabla \phi > $
\pagebreak

\[ V_(r,\sigma) = \exp \left( \log V_{int} C(r,\sigma) + \log V_{ext} (1 - C(r,\sigma) \right) = V_{ext} \exp \left( \log \frac{V_{int}}{V_{ext}} C(r,\sigma) \right) = V_{int} \exp \left( \log \frac{V_{ext}}{V_{int}} \overline{C}(r,\sigma) \right) \]
\pagebreak

$ C(r,\sigma) $
\pagebreak

$ \overline{C} $
\pagebreak

\[ \nabla \log V = \frac{\nabla V}{V} = \log \frac{V_{int}}{V_{ext}} \nabla C \]
\pagebreak

$ \nabla C $
\pagebreak

$ \| V_{ext} - V_{int} \| $
\pagebreak

$ C $
\pagebreak

$ \sigma $
\pagebreak

$ \nabla \log \epsilon $
\pagebreak

\begin{eqnarray*} u_t - u \cdot \nabla u + \nabla p & = &\mu \Delta u + f \\ \nabla \cdot u & = & 0 \end{eqnarray*}
\pagebreak

$ f $
\pagebreak

$ \mu $
\pagebreak

$ n+1 $
\pagebreak

\[ \Delta p = \nabla \cdot (f - u_{n} \cdot \nabla u_{n} ) \]
\pagebreak

$p$
\pagebreak

\[ (\frac{1}{ \delta t \mu } - \Delta) u_{n+1} = \frac {f - \nabla p - u_n \cdot \nabla u_n }{ \mu } + \frac {u_n}{ \delta t \mu } \]
\pagebreak

$u_{n+1}$
\pagebreak

\[ -\nabla^2 \psi(x) + V(x) \psi(x) = E \psi(x) \]
\pagebreak

\[ V(x) = -a \exp(-b x^2) + \frac{c}{(n(x)+\eta)^{1/3}} - d n(x)^{5/3} + V_{\mbox{shift}} \]
\pagebreak

$ a $
\pagebreak

$ b $
\pagebreak

$ c $
\pagebreak

$ d $
\pagebreak

$ V_{\mbox{shift}} $
\pagebreak

\[ n(x) = \psi(x)^2 \]
\pagebreak

\[ \psi = - 2 G_{\mu} * \left ( V \psi \right) \]
\pagebreak

$ G_{\mu}$
\pagebreak

\[ \left( - \frac{d^2}{dx^2} + \mu^2 \right) G(x,x^{\prime}) = \delta(x-x^{\prime}) \]
\pagebreak

$ \eta $
\pagebreak

$r(u) = 0$
\pagebreak

\[ \int_0^{10} sin(x) dx \]
\pagebreak

$ sin(x) $
\pagebreak

$ u(0) $
\pagebreak

\[ \frac{du}{dt} = \hat{L} u + N(u) \]
\pagebreak

$ t $
\pagebreak

$ u(t) $
\pagebreak

$ \hat{L} $
\pagebreak

$ N $
\pagebreak

\[ u(t) = \exp(t \hat{L} ) u(0) + \int_0^t \exp((t-\tau)\hat{L}) N(u(\tau)) d\tau \]
\pagebreak

$ n $
\pagebreak

$ O\left(t^{2n+1}\right) $
\pagebreak

$ 1+(n_{it}+1)n +n_{it}n^2 $
\pagebreak

$ n_{it} $
\pagebreak

$ t+\Delta $
\pagebreak

$ \exp{\tau \hat{L}} u $
\pagebreak

$ \tau \in (0,\Delta) $
\pagebreak

$ T \in (t,t+\Delta) $
\pagebreak

$ u $
\pagebreak

$ T $
\pagebreak

\[ -\nabla^2 \psi(x,t) + V(x,t) \psi(x,t) = i\psi_t(x,t) \]
\pagebreak

\[ V(x,t) = -8 \exp((x - v \cdot t)^2) \]
\pagebreak

$ v $
\pagebreak

\[ \psi(x,t) = \psi(x,0) * G(x,t) - \int_0^t V(x,s) \cdot \psi(x,s) * G(x,t-s) ds \]
\pagebreak

$ G $
\pagebreak

\[ \left( - \frac{d^2}{dx^2} - i \frac{d}{dt} \right) G(x) = \delta(x)). \]
\pagebreak

$ \psi(x,t) $
\pagebreak

$n$
\pagebreak

$ [0,t] $
\pagebreak

$ \psi $
\pagebreak

\[ \psi^{m+1}(x,t) - \psi^{m}(x,t) = - \int_0^t V(x,s) \cdot ( \psi^{m}(x,s) - \psi^{m-1}(x,s)) * G(x,t-s) ds \]
\pagebreak

\[ \delta^{m+1}(x,t) = - \int_0^t V(x,s) \cdot \delta^{m}(x,s) * G(x,t-s) ds \]
\pagebreak

$ \delta^m $
\pagebreak

$ m_{th} $
\pagebreak

$t$
\pagebreak

$ \nabla $
\pagebreak

$0 <= \mbox{mask(sdf)} <= 1$
\pagebreak

\[ \varphi(d) = \frac{1}{2}\left( 1 - \tanh\left( \frac{3d}{\varepsilon} \right) \right) \]
\pagebreak

$d$
\pagebreak

\[ B(\varphi) = \frac{36}{\varepsilon} \varphi^2 (1-\varphi)^2. \]
\pagebreak

$36/\varepsilon$
\pagebreak

\[ \int_{-\infty}^\infty B(s) \, ds = 1 \]
\pagebreak

$ |8 \epsilon| $
\pagebreak

$ \epsilon $
\pagebreak

\[ \int_{-\epsilon/2}^{\epsilon/2} B(s) \, ds \doteq 0.987 \]
\pagebreak

\[ \int_{-\epsilon}^{\epsilon} B(s) \, ds \doteq 0.999963 \]
\pagebreak

\[ \sqrt{x^2 + y^2} - c * z = 0 \]
\pagebreak

$ z $
\pagebreak

\[ x^2 + y^2 - c * z == 0 \]
\pagebreak

\[ \mathbf{C} \leftarrow \alpha \mathbf{A}^{\mathrm{OpA}} \mathbf{B}^{\mathrm{OpB}} + \beta \mathbf{C} \]
\pagebreak

$ \mathbf{A} $
\pagebreak

$ \mathbf{B} $
\pagebreak

$ \mathbf{C} $
\pagebreak

\[ \mathbf{y} \leftarrow \alpha \mathbf{A}^{\mathrm{OpA}} \mathbf{x} + \beta \mathbf{y} \]
\pagebreak

$ \mathbf{x} $
\pagebreak

$ \mathbf{y} $
\pagebreak

\[ \mathbf{A} \leftarrow \alpha \mathbf{x} \mathbf{y}^{\mathrm{T}} + \mathbf{A} \]
\pagebreak

$ \mathbf{x} \mathbf{y}^{\mathrm{T}} $
\pagebreak

\[ u \leftarrow \alpha \mathbf{x} \cdot \mathbf{y} \]
\pagebreak

\[ \mathbf{x} \leftarrow \alpha \mathbf{x} \]
\pagebreak

$ \mathbf{A} \vec{x} = \vec{b} $
\pagebreak

$\mathbf{A}$
\pagebreak

$\vec{b}$
\pagebreak

$\vec{x}$
\pagebreak

$||\mathbf{A} \vec{x} - \vec{b}||$
\pagebreak

$|| \vec{x}_{iter} - \vec{x}_{iter-1}||$
\pagebreak

\[ \vec{x} \leftarrow c \vec{x} \]
\pagebreak

\[ \vec{x} \leftarrow a \vec{x} + b \vec{y} \]
\pagebreak

$ f(x)=0 $
\pagebreak

$ j $
\pagebreak

$ m $
\pagebreak

\begin{eqnarray*} Q_{i j} & = & \langle x_i \mid f_j \rangle \\ A_{i j} & = & \langle x_i - x_m \mid f_j - f_m \rangle = Q_{i j} - Q_{m j} - Q_{i m} + Q{m m} \\ b_i & =& -\langle x_i - x_m \mid f_m \rangle = -Q_{i m} + Q_{m m} \end{eqnarray*}
\pagebreak

\[ A c = b \]
\pagebreak

\[ c_m = 1 - \sum_{i<m} c_i \]
\pagebreak

\[ x_{m+1} = \sum_{i \le m}{c_i ( x_i - f_i)} \]
\pagebreak

$ Q $
\pagebreak

$ x_i $
\pagebreak

$ f_j $
\pagebreak

$ R(*,*,\ldots) \rightarrow I(*,*,\ldots) $
\pagebreak

$ R(*) \rightarrow I(i,*) $
\pagebreak

$ ||v||_2 = \sqrt{\sum_{k=1}^N v_i^2} $
\pagebreak

\end{document}
